\[
\begin{aligned}
R_{1,1} &= c_{1,1} - u_{1} - v_{1} = 15 - 0 - 10 = 5 \\
R_{1,2} &= c_{1,2} - u_{1} - v_{2} = 18 - 0 - 10 = 8 \\
R_{1,3} &= c_{1,3} - u_{1} - v_{3} = 12 - 0 - 12 = 0 \\
R_{1,4} &= c_{1,4} - u_{1} - v_{4} = 13 - 0 - 13 = 0 \\
R_{1,5} &= c_{1,5} - u_{1} - v_{5} = 0 - 0 - 0 = 0 
R_{2,1} &= c_{2,1} - u_{2} - v_{1} = 10 - 0 - 10 = 0 \\
R_{2,2} &= c_{2,2} - u_{2} - v_{2} = 10 - 0 - 10 = 0 \\
R_{2,3} &= c_{2,3} - u_{2} - v_{3} = 11 - 0 - 12 = -1 \\
R_{2,4} &= c_{2,4} - u_{2} - v_{4} = 9 - 0 - 13 = -4 \\
R_{2,5} &= c_{2,5} - u_{2} - v_{5} = 0 - 0 - 0 = 0 
R_{3,1} &= c_{3,1} - u_{3} - v_{1} = 8 - -5 - 10 = 3 \\
R_{3,2} &= c_{3,2} - u_{3} - v_{2} = 5 - -5 - 10 = 0 \\
R_{3,3} &= c_{3,3} - u_{3} - v_{3} = 7 - -5 - 12 = 0 \\
R_{3,4} &= c_{3,4} - u_{3} - v_{4} = 8 - -5 - 13 = 0 \\
R_{3,5} &= c_{3,5} - u_{3} - v_{5} = 0 - -5 - 0 = 5 
\end{aligned}
\]

