\[
\begin{aligned}
R_{1,1} &= c_{1,1} - u_{1} - v_{1} = 3 - 0 - 3 = 0 \\
R_{1,2} &= c_{1,2} - u_{1} - v_{2} = 5 - 0 - 1 = 4 \\
R_{1,3} &= c_{1,3} - u_{1} - v_{3} = 7 - 0 - -4 = 11 \\
R_{1,4} &= c_{1,4} - u_{1} - v_{4} = 10 - 0 - 2 = 8 
R_{2,1} &= c_{2,1} - u_{2} - v_{1} = 6 - 3 - 3 = 0 \\
R_{2,2} &= c_{2,2} - u_{2} - v_{2} = 8 - 3 - 1 = 4 \\
R_{2,3} &= c_{2,3} - u_{2} - v_{3} = 13 - 3 - -4 = 14 \\
R_{2,4} &= c_{2,4} - u_{2} - v_{4} = 5 - 3 - 2 = 0 
R_{3,1} &= c_{3,1} - u_{3} - v_{1} = 4 - 1 - 3 = 0 \\
R_{3,2} &= c_{3,2} - u_{3} - v_{2} = 2 - 1 - 1 = 0 \\
R_{3,3} &= c_{3,3} - u_{3} - v_{3} = 6 - 1 - -4 = 9 \\
R_{3,4} &= c_{3,4} - u_{3} - v_{4} = 7 - 1 - 2 = 4 
R_{4,1} &= c_{4,1} - u_{4} - v_{1} = 12 - 8 - 3 = 1 \\
R_{4,2} &= c_{4,2} - u_{4} - v_{2} = 9 - 8 - 1 = 0 \\
R_{4,3} &= c_{4,3} - u_{4} - v_{3} = 4 - 8 - -4 = 0 \\
R_{4,4} &= c_{4,4} - u_{4} - v_{4} = 10 - 8 - 2 = 0 
\end{aligned}
\]

