\[
\begin{aligned}
R_{1,1} &= c_{1,1} - u_{1} - v_{1} = 3 - 0 - 3 = 0 \\
R_{1,2} &= c_{1,2} - u_{1} - v_{2} = 5 - 0 - 1 = 4 \\
R_{1,3} &= c_{1,3} - u_{1} - v_{3} = 7 - 0 - -5 = 12 \\
R_{1,4} &= c_{1,4} - u_{1} - v_{4} = 10 - 0 - 1 = 9 
R_{2,1} &= c_{2,1} - u_{2} - v_{1} = 6 - 4 - 3 = -1 \\
R_{2,2} &= c_{2,2} - u_{2} - v_{2} = 8 - 4 - 1 = 3 \\
R_{2,3} &= c_{2,3} - u_{2} - v_{3} = 13 - 4 - -5 = 14 \\
R_{2,4} &= c_{2,4} - u_{2} - v_{4} = 5 - 4 - 1 = 0 
R_{3,1} &= c_{3,1} - u_{3} - v_{1} = 4 - 1 - 3 = 0 \\
R_{3,2} &= c_{3,2} - u_{3} - v_{2} = 2 - 1 - 1 = 0 \\
R_{3,3} &= c_{3,3} - u_{3} - v_{3} = 6 - 1 - -5 = 10 \\
R_{3,4} &= c_{3,4} - u_{3} - v_{4} = 7 - 1 - 1 = 5 
R_{4,1} &= c_{4,1} - u_{4} - v_{1} = 12 - 9 - 3 = 0 \\
R_{4,2} &= c_{4,2} - u_{4} - v_{2} = 9 - 9 - 1 = -1 \\
R_{4,3} &= c_{4,3} - u_{4} - v_{3} = 4 - 9 - -5 = 0 \\
R_{4,4} &= c_{4,4} - u_{4} - v_{4} = 10 - 9 - 1 = 0 
\end{aligned}
\]

